OwlLean/TypeChecker/TcSimple.lean
@@ -68,22 +68,6 @@ theorem Owl.ty.simplify_rec_sound (phi : phi_context l) (psi : psi_context l) de
   -/
 
 
-
-
-
-
-
-
-
-
-
-
-
-
-
-
-
-
 namespace OwlTc
 
 
@@ -92,17 +76,18 @@ abbrev RCtx n := List (prop n 0)
 
 inductive SideCondition r where
   | PhiEntails : phi_context_repr l -> Owl.constr l -> SideCondition r
-  | PhiPsiEntailCorr : String -> phi_context_repr l -> psi_context l -> label l -> SideCondition r
+  | PhiPsiEntailCorr : String -> phi_context_repr l -> psi_context l -> corruption l -> SideCondition r
   | TyVarEq : Fin d -> Fin d -> SideCondition r
   | TyEq : ty l r d m -> ty l r d m -> SideCondition r
   | CondSymEq : cond_sym -> cond_sym -> SideCondition r
   | PsiContextInconsistent : String -> phi_context_repr l -> psi_context l -> SideCondition r
   | RexpEq : rexp r 0 -> rexp r 0 -> SideCondition r
   | PropHolds : prop r 0 -> SideCondition r
+  | ScOr : SideCondition r -> SideCondition r -> SideCondition r
+  | ScAnd : SideCondition r -> SideCondition r -> SideCondition r
+  | ScTrue
+  | ScFalse
 deriving ToExpr
-
-instance : ToString (SideCondition r) where
-  toString := fun _ => "<sc>"
 
 
 @[simp]
@@ -136,13 +121,35 @@ def interp_prop (p : prop r 0) (bvar_interp : Fin r -> String) (fvar_interp : Le
 def SideCondition.eval (p : SideCondition r) (bvar_interp : Fin r -> String) (fvar_interp : Lean.Name -> String) (f_interp : String -> String -> String -> String) : Prop :=
   match p with
   | PhiEntails phi c => vec.to_fn phi |= c
-  | PhiPsiEntailCorr _ phi psi l => phi_psi_entail_corr (vec.to_fn phi) psi (.corr l)
+  | PhiPsiEntailCorr _ phi psi l => phi_psi_entail_corr (vec.to_fn phi) psi l
   | TyVarEq x y => x = y
   | TyEq t1 t2 => t1 = t2
   | CondSymEq c1 c2 => c1 = c2
   | PsiContextInconsistent _ phi psi => psi_context_inconsistent (vec.to_fn phi) psi
   | RexpEq re1 re2 => (rexp_interp re1 bvar_interp fvar_interp f_interp) = (rexp_interp re2 bvar_interp fvar_interp f_interp)
   | PropHolds p1 => interp_prop p1 bvar_interp fvar_interp f_interp
+  | ScOr e1 e2 => e1.eval bvar_interp fvar_interp f_interp ∨ e2.eval bvar_interp fvar_interp f_interp
+  | ScAnd e1 e2 => e1.eval bvar_interp fvar_interp f_interp ∧  e2.eval bvar_interp fvar_interp f_interp
+  | ScTrue => True
+  | ScFalse => False
+
+def SideCondition.pretty (p : SideCondition r) : String :=
+  match p with
+  | SideCondition.PhiEntails phi c => s!"({repr phi} |= {repr c})"
+  | SideCondition.PhiPsiEntailCorr msg phi psi co => s!"(phi, psi |= {repr co})"
+  | SideCondition.TyVarEq x y => s!"(TyVarEq {toString x} == {toString y})"
+  | SideCondition.TyEq t1 t2 => s!"(TyEq {toString t1} == {toString t2})"
+  | SideCondition.CondSymEq c1 c2 => s!"(CondSymEq {toString c1} == {toString c2})"
+  | SideCondition.PsiContextInconsistent msg phi psi => s!"(psi_context_inconsistent {msg})"
+  | SideCondition.RexpEq re1 re2 => s!"({repr re1} == {repr re2})"
+  | SideCondition.PropHolds p1 => s!"(PropHolds {repr p1})"
+  | SideCondition.ScOr e1 e2 => s!"({pretty e1} ∨ {pretty e2})"
+  | SideCondition.ScAnd e1 e2 => s!"({pretty e1} ∧ {pretty e2})"
+  | SideCondition.ScTrue => "True"
+  | SideCondition.ScFalse => "False"
+
+instance : ToString (SideCondition r) where
+  toString := SideCondition.pretty
 
 @[simp]
 def RCtx.interp (theta : RCtx r) (bvar_interp : Fin r -> String) (fvar_interp : Lean.Name -> String) (f_interp : String -> String -> String -> String) : Prop :=
@@ -159,99 +166,121 @@ structure SideConditionWithContext where
   sc : SideCondition r
   deriving ToExpr
 
-structure CheckContext M [Monad M] where
-  visitTm : forall l r d m, Owl.opaqueSyntax -> ty l r d m -> M Unit
-  log : String -> M Unit
-  fresh : M Lean.Name
+structure CheckContext  where
   curSyntax : Option Owl.opaqueSyntax
 
-inductive CheckOutput where
-  | true : CheckOutput
-  | sc : SideConditionWithContext -> CheckOutput
-  | and : CheckOutput -> CheckOutput -> CheckOutput
-  | or : CheckOutput -> CheckOutput -> CheckOutput
-  deriving ToExpr
-
-infixr:60 " ∧sc " => CheckOutput.and
-infixr:60 " ∨sc " => CheckOutput.or
-notation " ⊤ " => CheckOutput.true
 
 
+abbrev CheckContext.init : CheckContext := { curSyntax := none }
 
-@[simp]
-def CheckOutput.simpl (c : CheckOutput) : CheckOutput :=
-  match c with
-  | .true => .true
-  | .and e1 e2 =>
-      let e1' := e1.simpl
-      let e2' := e2.simpl
-      match e1', e2' with
-      | .true, _ => e2'
-      | _, .true => e1'
-      | _, _ => e1' ∧sc e2'
-  | .or e1 e2 =>
-      let e1' := e1.simpl
-      let e2' := e2.simpl
-      match e1', e2' with
-      | .true, _ => .true
-      | _, .true => .true
-      | _, _ => e1' ∨sc e2'
-  | .sc s => .sc s
-
-
-
-abbrev CheckContext.init [Monad M] (visit : forall l d r m, Owl.opaqueSyntax -> ty l d r m -> M Unit) (log : String -> M Unit) (fresh : M Lean.Name) : CheckContext M :=
-  { visitTm := visit, curSyntax := .none, log := log, fresh := fresh }
-
-abbrev CheckT m [Monad m] α :=
-  ReaderT (CheckContext m) m (Result (Option opaqueSyntax × String) (α × CheckOutput))
+abbrev CheckT (α : Type) :=
+  ReaderT CheckContext TermElabM (Result (Option opaqueSyntax × String) α)
 
 -- CheckState m -> m (Result (Option opaqueSyntax × String) (α × CheckState m))
 
 @[always_inline, simp]
-instance [Monad m] : Monad (CheckT m) where
-  pure := fun x => fun _ => pure (.ok (x, .true))
+instance : Monad CheckT where
+  pure := fun x => fun _ => pure (.ok x)
   bind := fun c k => fun ctx => do
     match <- (c ctx) with
     | .err e => pure (.err e)
-    | .ok (x, o1) => do
+    | .ok x => do
         match <- (k x ctx) with
         | .err e2 => pure (.err e2)
-        | .ok (res, o2) => pure $ .ok (res, o1.and o2)
+        | .ok (res) => pure $ .ok (res)
 
 
-def emit [Monad m] r (theta : RCtx r) (p : SideCondition r) : CheckT m Unit := fun _ =>
-  pure $ .ok ((), .sc $ ⟨r, theta, p⟩)
+opaque S : Type
+opaque T : Type
+opaque P : S -> T -> Prop
+opaque Q : S -> T -> Prop
+def foo : Prop := forall s t, P s t -> Q s t
 
-def withSyntax [Monad m] (s : Owl.opaqueSyntax) (k : CheckT m α) : CheckT m α :=
+attribute [simp] Fin.foldr_succ
+
+#check Fin.foldr_succ
+
+theorem tst : True := by
+  simp
+
+namespace Proof
+
+opaque owl_f_interp' : String -> String -> String -> String
+
+def owl_f_interp (s x y : String) : String :=
+  match s with
+  | "concat" => x ++ y
+  | _ => owl_f_interp' s x y
+
+@[simp]
+def SideConditionWithContext.eval (sc : SideConditionWithContext) : Prop :=
+  forall bv fv, RCtx.interp sc.theta bv fv owl_f_interp -> sc.sc.eval bv fv owl_f_interp
+
+def runGrind (g : Expr) : TermElabM Bool := do
+  let g <- mkFreshExprMVar g
+  let res <- Grind.main g.mvarId! (<- Grind.mkDefaultParams {})
+  return res.failure?.isNone
+
+
+def doSimp (e : Expr) : TermElabM Expr := do
+  let ctx <- Simp.Context.mkDefault
+  let res <- Lean.Meta.simp e ctx
+  return res.fst.expr
+
+
+ def doGrindSc {r} (theta : RCtx r) (sc : SideCondition r) : TermElabM Bool := do
+  let scc : SideConditionWithContext := {r := r, theta := theta, sc := sc}
+  let e  <- mkAppM ``SideConditionWithContext.eval #[toExpr scc]
+  let e <- doSimp e
+  -- logInfo s!"doGrindSc: simped to {<- PrettyPrinter.ppExpr e}"
+  runGrind e
+
+end Proof
+
+
+def prove r (theta : RCtx r) (p : SideCondition r) : CheckT Bool := fun _ => do
+  -- logInfo s!"Proving {p}"
+  let b <- Proof.doGrindSc theta p
+  -- logInfo s!"Got {b}"
+  pure $ .ok b
+
+def withSyntax (s : Owl.opaqueSyntax) (k : CheckT α) : CheckT α :=
   fun st => k {st with curSyntax := .some s}
 
 
-def throw [Monad m] (s : String) : CheckT m α := fun st => pure $ .err (st.curSyntax, s)
+def throw (s : String) : CheckT α := fun st => pure $ .err (st.curSyntax, s)
 
-def visit [Monad m] (s : Owl.opaqueSyntax) (t : ty l d r n) : CheckT m Unit := fun st => do
-  st.visitTm _ _ _ _ s t
-  pure (.ok ((), .true))
 
-def log [Monad m] (s : String) : CheckT m Unit := fun st => do
-  st.log s
-  pure (.ok ((), .true))
+def addTypeInfo (stx : Syntax) (s : String) := do
+    let n : Name := Name.mkSimple s
 
-def freshName [Monad m] : CheckT m Lean.Name := fun st => do
-  let i <- st.fresh
-  pure (.ok (i, .true))
+    withEnableInfoTree true do withLocalDeclD n (mkSort levelOne) fun dslType => do
+      let forgedExpr ← mkFreshExprMVar dslType
+      pushInfoLeaf <| .ofTermInfo {
+        elaborator := `Sequent
+        stx := stx
+        lctx := (← getLCtx)
+        expectedType? := some dslType
+        expr := forgedExpr
+        isBinder := false
+      }
+    pure ()
 
-def CheckT.or [Monad m] (c1 : CheckT m Unit) (c2 : CheckT m Unit) : CheckT m Unit :=
-  fun ctx => do
-    match <- c1 ctx with
-    | .err s => return .err s
-    | .ok (_, o1) => do
-      match <- c2 ctx with
-      | .err s => return .err s
-      | .ok (_, o2) => return .ok ((), o1.or o2)
+def visit (s : Owl.opaqueSyntax) (t : ty l d r n) : CheckT Unit := fun st => do
+  addTypeInfo s.inner (toString t)
+  pure (.ok ())
 
+def log  (s : String) : CheckT Unit := fun st => do
+  println! s
+  pure (.ok ())
+
+def freshName  : CheckT Lean.Name := fun st => do
+  let i <- mkFreshId
+  pure (.ok i)
 
 abbrev subtype_fuel := 10
+
+
 
 -- TODO : Finish up various cases that have not yet been completed (for check_subtype and infer)!
 
@@ -260,7 +289,7 @@ def lift_RCtx_r (r : RCtx n) : RCtx (n + 1) :=
   r.map (ren_prop shift id)
 
 
-partial def extract_refinements [Monad m] (t : ty l r d 0) : CheckT m (RCtx r × ty l r d 0) :=
+partial def extract_refinements (t : ty l r d 0) : CheckT (RCtx r × ty l r d 0) :=
   match t with
   | .ex_r t0 => do -- ∃ x. t
     let i <- freshName
@@ -278,100 +307,124 @@ partial def extract_refinements [Monad m] (t : ty l r d 0) : CheckT m (RCtx r ×
 
 
 
-def check_subtype  [Monad m] (fuel : Nat) (Phi : phi_context l) (Psi : psi_context l) (Delta : delta_context l r d )
+def check_subtype'  (fuel : Nat) (Phi : phi_context l) (Psi : psi_context l) (Delta : delta_context l r d )
                            (Theta : RCtx r)
-                           (t1 : ty l r d 0) (t2 : ty l r d 0) : CheckT m Unit := do
+                           (t1 : ty l r d 0) (t2 : ty l r d 0) : CheckT (SideCondition r) := do
     -- log s!"check subtype: {t1} <= {t2}"
-    if t1 == t2 then pure () else
+    if t1 == t2 then pure .ScTrue else
     match fuel with
-    | 0 => throw "check_subtype: out of fuel"
+    | 0 => throw "check_subtype': out of fuel"
     | (n + 1) =>
       match t1, t2 with
-      | .admit, _ => pure ()
-      | _, .Any => pure ()
-      | .Unit, .Unit => pure ()
+      | .admit, _ => pure .ScTrue
+      | _, .Any => pure .ScTrue
+      | .Unit, .Unit => pure .ScTrue
       | _, .refined t p => do
-        check_subtype n Phi Psi Delta Theta t1 t
-        emit r Theta (.PropHolds p)
+        let r1 <- check_subtype' n Phi Psi Delta Theta t1 t
+        pure $ r1.ScAnd $ .PropHolds p
       | _, .inter t21 t22 => do
-        check_subtype n Phi Psi Delta Theta t1 t21
-        check_subtype n Phi Psi Delta Theta t1 t22
+        let r1 <- check_subtype' n Phi Psi Delta Theta t1 t21
+        let r2 <- check_subtype' n Phi Psi Delta Theta t1 t22
+        pure $ .ScAnd r1 r2
       | _, .union t21 t22 => do
-        CheckT.or (check_subtype n Phi Psi Delta Theta t1 t21)
-                  (check_subtype n Phi Psi Delta Theta t1 t22)
+        let r1 <- (check_subtype' n Phi Psi Delta Theta t1 t21)
+        let r2 <- (check_subtype' n Phi Psi Delta Theta t1 t22)
+        pure $ .ScOr r1 r2
       | .inter t11 t12, _ =>
-        CheckT.or (check_subtype n Phi Psi Delta Theta t11 t2)
-                  (check_subtype n Phi Psi Delta Theta t12 t2)
+        let r1 <- (check_subtype' n Phi Psi Delta Theta t11 t2)
+        let r2 <- (check_subtype' n Phi Psi Delta Theta t12 t2)
+        pure $ .ScOr r1 r2
       | .RData l1 _, .Data l2 =>
-        emit r Theta (.PhiEntails (vec.from_fn Phi) (.condition .leq l1 l2))
+        pure $ (.PhiEntails (vec.from_fn Phi) (.condition .leq l1 l2))
       | .RData l1 re1, .RData l2 re2 => do
-        emit r Theta (.PhiEntails (vec.from_fn Phi) (.condition .leq l1 l2))
-        emit r Theta (.RexpEq re1 re2)
-        pure ()
+        let r1 := (SideCondition.PhiEntails (vec.from_fn Phi) (.condition .leq l1 l2))
+        let r2 := (.RexpEq re1 re2)
+        pure $ r1.ScAnd r2
       | .Data l1, .Public => do
-        emit r Theta (.PhiPsiEntailCorr s!"Data {l1}, Public" (vec.from_fn Phi) Psi l1)
+        pure $ (.PhiPsiEntailCorr s!"Data {l1}, Public" (vec.from_fn Phi) Psi (.corr l1))
       | .RData l1 _, .Public => do
-        emit r Theta (.PhiPsiEntailCorr s!"RData {l1}, Public" (vec.from_fn Phi) Psi l1)
-        pure ()
+        pure (.PhiPsiEntailCorr s!"RData {l1}, Public" (vec.from_fn Phi) Psi (.corr l1))
       | .Data l1, ty.ex_r (.RData l2 (.var 0)) =>
-        emit r Theta (.PhiEntails (vec.from_fn Phi) (.condition .leq l1 l2))
+        pure (.PhiEntails (vec.from_fn Phi) (.condition .leq l1 l2))
       | .var_ty x1, .var_ty x2 =>
-        emit r Theta (.TyVarEq x1 x2)
-      | .Public, .Public => pure ()
-      | .var_ty x, t' => check_subtype n Phi Psi Delta Theta (Delta x) t'
-      | t, .var_ty x => check_subtype n Phi Psi Delta Theta t (Delta x)
+        pure (.TyVarEq x1 x2)
+      | .Public, .Public => pure .ScTrue
+      | .var_ty x, t' => check_subtype' n Phi Psi Delta Theta (Delta x) t'
+      | t, .var_ty x => check_subtype' n Phi Psi Delta Theta t (Delta x)
       -- | .Public, .Data _ => pure ()
       | (.arr t1 t2), (.arr t1' t2') => do
-        check_subtype n Phi Psi Delta Theta t1' t1
-        check_subtype n Phi Psi Delta Theta t2 t2'
+        let r1 <- check_subtype' n Phi Psi Delta Theta t1' t1
+        let r2 <- check_subtype' n Phi Psi Delta Theta t2 t2'
+        pure $ r1.ScAnd r2
       | (.prod t1 t2), (.prod t1' t2') => do
-        check_subtype n Phi Psi Delta Theta t1 t1'
-        check_subtype n Phi Psi Delta Theta t2 t2'
+        let r1 <- check_subtype' n Phi Psi Delta Theta t1 t1'
+        let r2 <- check_subtype' n Phi Psi Delta Theta t2 t2'
+        pure $ r1.ScAnd r2
       | (.sum t1 t2), (.sum t1' t2') => do
-        check_subtype n Phi Psi Delta Theta t1 t1'
-        check_subtype n Phi Psi Delta Theta t2 t2'
+        let r1 <- check_subtype' n Phi Psi Delta Theta t1 t1'
+        let r2 <- check_subtype' n Phi Psi Delta Theta t2 t2'
+        pure $ r1.ScAnd r2
       | .Ref u, .Ref v =>
-        emit r Theta (.TyEq u v)
+        pure $ (.TyEq u v)
       | .all t0 t, .all t0' t' => do
-        check_subtype n Phi Psi Delta Theta t0 t0'
+        let r1 <- check_subtype' n Phi Psi Delta Theta t0 t0'
         let extended_delta := lift_delta (cons t0' Delta)
-        check_subtype n Phi Psi extended_delta Theta t t'
+        let r2 <- check_subtype' n Phi Psi extended_delta Theta t t'
+        pure $ r1.ScAnd r2
       | .ex t0 t, .ex t0' t' => do
-        check_subtype n Phi Psi Delta Theta t0 t0'
+        let r1 <- check_subtype' n Phi Psi Delta Theta t0 t0'
         let extended_delta := lift_delta (cons t0 Delta)
-        check_subtype n Phi Psi extended_delta Theta t t'
+        let r2 <- check_subtype' n Phi Psi extended_delta Theta t t'
+        pure $ r1.ScAnd r2
       | .all_l cs lab t, .all_l cs' lab' t' => do
         let extended_phi := lift_phi (cons (cs, lab) Phi)
         let constraint := (.condition cs (.var_label "_" var_zero) (ren_label shift lab'))
         -- let constraint_holds := extended_phi |= constraint
-        emit r Theta (.PhiEntails (vec.from_fn extended_phi) constraint)
+        let r1 := (SideCondition.PhiEntails (vec.from_fn extended_phi) constraint)
         let extended_psi := lift_psi Psi
         let extended_delta := lift_delta_l Delta
-        check_subtype n extended_phi extended_psi extended_delta Theta t t'
-        emit r Theta (.CondSymEq cs cs')
+        let r2 <- check_subtype' n extended_phi extended_psi extended_delta Theta t t'
+        pure $ r1.ScAnd r2
       | .t_if lab t1 t2, t' => do
-        check_subtype n Phi ((.corr lab) :: Psi) Delta Theta t1 t'
-        check_subtype n Phi ((.not_corr lab) :: Psi) Delta Theta t2 t'
+        let r1 <- check_subtype' n Phi ((.corr lab) :: Psi) Delta Theta t1 t'
+        let r2 <- check_subtype' n Phi ((.not_corr lab) :: Psi) Delta Theta t2 t'
+        pure $ r1.ScAnd r2
       | t, .t_if lab t1' t2' => do
-        check_subtype n Phi ((.corr lab) :: Psi) Delta Theta t t1'
-        check_subtype n Phi ((.not_corr lab) :: Psi) Delta Theta t t2'
+        let r1 <- check_subtype' n Phi ((.corr lab) :: Psi) Delta Theta t t1'
+        let r2 <- check_subtype' n Phi ((.not_corr lab) :: Psi) Delta Theta t t2'
+        pure $ r1.ScAnd r2
       | _, _ =>
-        let s := s!"Could not prove {repr t1} <: {repr t2}"
-        emit r Theta (.PsiContextInconsistent s (vec.from_fn Phi) Psi)
-        -- throw s!"check_subtype: cannot prove {t1.pretty} <= {t2.pretty}}"
+        pure (.PsiContextInconsistent s!"check_subtype': {t1} and {t2} are not comparable" (vec.from_fn Phi) Psi)
 
+def check_subtype (fuel : Nat) (Phi : phi_context l) (Psi : psi_context l) (Delta : delta_context l r d)
+                           (Theta : RCtx r)
+                           (t1 : ty l r d 0) (t2 : ty l r d 0) : CheckT Unit := do
+  let sc <- check_subtype' fuel Phi Psi Delta Theta t1 t2
+  let b <- prove _ Theta sc
+  if b then pure ()
+       else throw $ s!"Could not prove {repr t1} <: {repr t2}"
 
 @[simp]
-def from_synth [Monad m] (Phi : phi_context l) (Psi : psi_context l) (Delta : delta_context l r d)
+def from_synth  (Phi : phi_context l) (Psi : psi_context l) (Delta : delta_context l r d)
           (Theta : RCtx r)
           (t : ty l r d 0) (exp : Option (ty l r d 0)) :
-          CheckT m (ty l r d 0) :=
+          CheckT (ty l r d 0) :=
     match exp with
     | .none => pure t
     | .some t' => do
       check_subtype subtype_fuel Phi Psi Delta Theta t t'
       pure t'
 
+
+def check_corrupt  (Phi : phi_context l) (Psi : psi_context l)
+          (Theta : RCtx r) (l : label l) : CheckT (Option Bool) := do
+    if Psi.contains (.corr l) then pure (.some True)
+    else if <- prove _ Theta (.PhiPsiEntailCorr s!"check_corrupt" (vec.from_fn Phi) Psi (.corr l))
+    then pure (.some True)
+    else if Psi.contains (.not_corr l) then pure (.some False)
+    else if <- prove _ Theta (.PhiPsiEntailCorr s!"check_corrupt" (vec.from_fn Phi) Psi (.not_corr l))
+    then pure (.some False)
+    else pure (.none)
 
 /-
 
@@ -392,14 +445,15 @@ def from_synth [Monad m] (Phi : phi_context l) (Psi : psi_context l) (Delta : de
 -- If no type is provided, infer will attempt to synthesize the type of the input term
 -- If successful, it will return the synthesized type, and a proof that the input term has that type
 
-def infer_op [Monad M] (Theta : RCtx r) (Phi : phi_context l) (op : String) (t1 : ty l r d 0) (t2 : ty l r d 0) : CheckT M (ty l r d 0) :=
+def infer_op (Theta : RCtx r) (Phi : phi_context l) (op : String) (t1 : ty l r d 0) (t2 : ty l r d 0) : CheckT (ty l r d 0) :=
   match t1, t2 with
   | .RData l1 r1, .RData l2 r2 => do
-      emit r Theta (.PhiEntails (vec.from_fn Phi) (.condition .leq l2 l1))
-      return (.RData l1 (.op op r1 r2))
+      let b <- prove _ Theta (.PhiEntails (vec.from_fn Phi) (.condition .leq l2 l1))
+      if b then pure (.RData l1 (.op op r1 r2))
+           else throw "infer_op: could not prove Phi |= l2 <= l1"
   | .Public, .Public => return .Public
   | _, _ => do
-    let getLabel (t : ty l r d 0) : CheckT M (label l) :=
+    let getLabel (t : ty l r d 0) : CheckT (label l) :=
       match t with
       | .Public => return .latl L.bot
       | .RData l _ => return l
@@ -409,13 +463,13 @@ def infer_op [Monad M] (Theta : RCtx r) (Phi : phi_context l) (op : String) (t1 
     let l2 <- getLabel t2
     return (.Data (label.ljoin l1 l2))
 
-def resolve_ty [Monad M] (Gamma : gamma_context l r d n) (t : ty l r d n) : CheckT M (ty l r d 0) :=
+def resolve_ty (Gamma : gamma_context l r d n) (t : ty l r d n) : CheckT (ty l r d 0) :=
   t.resolve_tm fun i =>
     match (Gamma i) with
     | ty.RData _ a => return a
     | _ => throw s!"Refinement expression or prop cannot make reference to non-refinfed variable"
 
-def resolve_re [Monad M] (Gamma : gamma_context l r d n) (t : rexp r n) : CheckT M (rexp r 0) :=
+def resolve_re (Gamma : gamma_context l r d n) (t : rexp r n) : CheckT (rexp r 0) :=
   t.resolve_tm fun i =>
     match (Gamma i) with
     | ty.RData _ a => return a
@@ -423,10 +477,10 @@ def resolve_re [Monad M] (Gamma : gamma_context l r d n) (t : rexp r n) : CheckT
 
 
 mutual
-def infer [Monad M] (Phi : phi_context l) (Psi : psi_context l) (Delta : delta_context l r d)
+def infer (Phi : phi_context l) (Psi : psi_context l) (Delta : delta_context l r d)
           (Theta : RCtx r)
           (Gamma : gamma_context l r d m) (e : tm l r d m) (exp : Option (ty l r  d 0)) :
-          CheckT M (ty l r  d 0) :=
+          CheckT (ty l r  d 0) :=
       match e with
       | .mk stx v => do
         let t <- withSyntax stx $ inferX Phi Psi Delta Theta Gamma v exp
@@ -434,10 +488,10 @@ def infer [Monad M] (Phi : phi_context l) (Psi : psi_context l) (Delta : delta_c
         visit stx t
         return t
 
-def inferX [Monad M] (Phi : phi_context l) (Psi : psi_context l) (Delta : delta_context l r d)
+def inferX (Phi : phi_context l) (Psi : psi_context l) (Delta : delta_context l r d)
           (Theta : RCtx r)
           (Gamma : gamma_context l r d m) (e : tmX l r d m) (exp : Option (ty l r  d 0)) :
-          CheckT M (ty l r  d 0) :=
+          CheckT (ty l r  d 0) :=
   match e with
   | .admit => from_synth Phi Psi Delta Theta .admit exp
   | .var_tm x =>
@@ -621,7 +675,9 @@ def inferX [Monad M] (Phi : phi_context l) (Psi : psi_context l) (Delta : delta_
       match <- infer Phi Psi Delta Theta Gamma e .none with
       | .all_l cs lab t  => do
         let result_ty := subst_ty (cons lab' (.var_label "_")) .var .var_ty t
-        emit r Theta (.PhiEntails (vec.from_fn Phi) (.condition cs lab lab'))
+        let b <- prove _ Theta (.PhiEntails (vec.from_fn Phi) (.condition cs lab lab'))
+        if b then pure result_ty
+             else throw "lapp: could not prove Phi |= cs lab lab'"
         pure result_ty
       | _ => throw "lapp"
     | .some exp_ty => do
@@ -629,7 +685,9 @@ def inferX [Monad M] (Phi : phi_context l) (Psi : psi_context l) (Delta : delta_
       | .all_l cs lab t => do
         let result_ty := subst_ty (cons lab' (.var_label "_")) .var .var_ty t
         check_subtype subtype_fuel Phi Psi Delta Theta result_ty exp_ty
-        emit r Theta (.PhiEntails (vec.from_fn Phi) (.condition cs lab lab'))
+        let b <- prove _ Theta (.PhiEntails (vec.from_fn Phi) (.condition cs lab lab'))
+        if b then pure exp_ty
+             else throw "lapp: could not prove Phi |= cs lab lab'"
         pure exp_ty
       | _ => throw "lapp"
   | .annot e t' => do
@@ -640,20 +698,17 @@ def inferX [Monad M] (Phi : phi_context l) (Psi : psi_context l) (Delta : delta_
     let t1 <- infer Phi ((.corr lab) :: Psi) Delta Theta Gamma e1 none
     let t2 <- infer Phi ((.not_corr lab) :: Psi) Delta Theta Gamma e2 none
     from_synth Phi Psi Delta Theta (.t_if lab t1 t2) exp
-  | .corr_case lab e =>
-    match exp with
+  | .corr_case lab e => do
+    match <- check_corrupt Phi Psi Theta lab with
     | .none => do
       let psi_corr := (.corr lab) :: Psi
       let psi_not_corr := (.not_corr lab) :: Psi
-      let t1 <- infer Phi psi_corr Delta Theta Gamma e .none
-      let t2 <- infer Phi psi_not_corr Delta Theta Gamma e .none
-      pure (.t_if lab t1 t2)
-    | .some exp_ty =>do
-      let psi_corr := (.corr lab) :: Psi
-      let psi_not_corr := (.not_corr lab) :: Psi
-      let _ <- infer Phi psi_corr Delta Theta Gamma e (.some exp_ty)
-      let _ <- infer Phi psi_not_corr Delta Theta Gamma e (.some exp_ty)
-      pure exp_ty
+      let t1 <- infer Phi psi_corr Delta Theta Gamma e exp
+      let t2 <- infer Phi psi_not_corr Delta Theta Gamma e exp
+      match exp with
+      | .none => pure (.t_if lab t1 t2)
+      | .some exp_ty => pure exp_ty
+    | .some _ => infer Phi Psi Delta Theta Gamma e exp
   | .sync e => do
     let _ <- infer Phi Psi Delta Theta Gamma e (.some .Public)
     from_synth Phi Psi Delta Theta .Public exp
@@ -671,21 +726,6 @@ def delabTypeError : Unexpander
   | `($_typeerror $_o $s) => set_option hygiene false in `(type error $s)
   | _ => set_option hygiene false in `(bad)
 
-
--- def has_type_infer M [Monad M] (visit : forall l r d, Owl.opaqueSyntax -> ty l r d -> M Unit)
---    (Phi : phi_context l) (Psi : psi_context l) (Delta : delta_context l r d)
---     (Gamma : gamma_context l r d m) (e : tm l r d m) (exp : ty l r d) : M (Result Prop (List SideCondition)) := do
---   match <- (infer Phi Psi Delta Gamma e (.some exp)) (CheckState.init visit (fun _ => pure ())) with
---   | .ok (_, p) => pure $ .ok $ p.side_condition
---   | .err e => pure $ .err $ TypeError e.1 e.2
-
--- Useful TODO
-/-
-theorem infer_sound Phi Psi Delta Gamma (e : tm l d m) (exp : ty l d) :
-  has_type_infer Id (fun _ _ _ _ => ()) Phi Psi Delta Gamma e exp ->
-  has_type Phi Psi Delta Gamma e exp := by
-    sorry
--/
 
 syntax "split_grind" : tactic
 
